more confusions

src/notes.lean
@@ -1,8 +1,17 @@
+
 /- These are some notes on confusing things in lean. 
-
-Let's look at equality first.  Here is a (renamed) version of the definition of equality.
-
+First, we set some options to illuminate implicit arguments.
 -/
+
+
+set_option pp.implicit true
+set_option pp.notation false 
+
+/-
+Let's look at equality first.  Here is a (renamed) version of the definition of equality.
+-/
+
+
 universe u
 
 inductive jteq {α : Sort u} (a : α): α → Prop 
@@ -50,7 +59,6 @@ In our case this means that jteq.refl a is a term whose type is jteq a a.
 
 
 
-
 /- 
 In the language of propositions as types and proofs as terms, this means we have a *proof* of the proposition
 that jteq a a for any type α and any a of that type. This is a sort of universal reflexivity.
@@ -61,7 +69,7 @@ that jteq a a for any type α and any a of that type. This is a sort of universa
 -/
 
 #check @jteq.rec
--- jteq.rec : Π {α : Sort u_2} {a : α} {C : α → Sort u_1}, C a → Π {ᾰ : α}, jteq a ᾰ → C ᾰ
+-- jteq.rec : Π {α : Sort u_2} {a : α} {C : α → Sort u_1}, C a → Π {ᾰ : α}, @jteq a ᾰ → C ᾰ
 /- 
 This takes as arguments a type α, a term a of that type, and a function that takes terms of type α
 to a (potentially) different type.
@@ -82,21 +90,19 @@ In the special case where C: α → Prop is a predicate, this says:
 We can put this in the form of a theorem, following Buzzard's blog post on induction on equality. 
 -/
 
-def jtr {α : Sort u} (a b : α) := jteq b a
+def jtr {α : Sort u} (a b : α) := λ (a b : α), jteq b a
 
 theorem jteq.subst {α : Sort u} {r s: α} (P : α → Prop) (h₁ : jteq r s) (h₂ : P r) : P s :=
 @jteq.rec α r P h₂ s h₁
 
-theorem jteq.subst2 {α : Sort u} {r s: α} (P : α → Prop) (h₁ : jteq r s) (h₂ : P r) : P s :=
-jteq.rec h₂ h₁
+
 /- Amazingly this is sufficient to show that jteq is symmetric and transitive.
 -/
 
 theorem jteq.symm {α : Sort u} {a b : α} (h : jteq a b) : jteq b a  :=
 @jteq.subst α a b (λ b, jteq b a) h (@jteq.refl α a) 
 
-theorem jteq.symm2 {α : Sort u} {a b : α} (h : jteq a b) : jteq b a  :=
-@jteq.subst α a b (λ b, jteq b a) h (@jteq.refl α a) 
+
 /- 
 To decode this proof, notice that our predicate is jteq _ a, so P a  is jteq a a  and P b is jteq b a
 So P a is true by reflexivity and P a with a=b → P b  which is b=a.
@@ -121,13 +127,24 @@ We want jteq b a, so we switch h₁, and then we need to switch the order of the
 -/
 
 theorem jteq.trans {α : Sort u} (a b c :α) (h₁ : jteq a b) (h₂ : jteq b c) : jteq a c:=
-@jteq.subst α b a (λ x, jteq x c) (@jteq.symm α a b h₁) (h₂)
+@jteq.subst α b a (λ x, @jteq α x c) (@jteq.symm α a b h₁) (h₂)
 
 
+namespace hidden
 
+inductive eq2 {α : Sort u} (a : α) : α → Prop
+| refl [] : eq2 a
 
+@[pattern] def rfl {α : Sort u} {a : α} : eq2 a a := eq2.refl a
 
-inductive jteq2 {α : Sort u} : α → α → Prop 
-| refl (a : α) : jteq2 a a 
+@[elab_as_eliminator, subst]
+lemma eq2.subst {α : Sort u} {P : α → Prop} {a b : α} (h₁ : eq2 a b) (h₂ : P a) : P b :=
+eq2.rec h₂ h₁
 
+@[trans] lemma eq2.trans {α : Sort u} {a b c : α} (h₁ : eq2 a b) (h₂ : eq2 b c) : eq2 a c:=
+eq2.subst h₂  h₁
 
+@[symm] lemma eq2.symm {α : Sort u} {a b : α} (h : eq2 a b) : eq2 b a :=
+eq2.subst h rfl 
+
+end hidden
